Refinery.lean
@@ -4,3 +4,5 @@ import Refinery.Term.Extrinsic.Semantics.Typing
 import Refinery.Term.Extrinsic.Subst
 import Refinery.Term.Extrinsic.Semantics.Wk
 import Refinery.Term.Extrinsic.Semantics.Minimal
+import Refinery.Term.Extrinsic.Refinement.Uniform
+import Refinery.Term.Extrinsic.Refinement.Semantics.Uniform
