Refinery/Term/Extrinsic/Refinement/Semantics/Uniform.lean
@@ -1,0 +1,30 @@
+import Refinery.Term.Extrinsic.Refinement.Uniform
+import Refinery.Term.Extrinsic.Semantics.Typing
+
+namespace Refinery
+
+open CategoryTheory
+
+open MonoidalCategory' PremonoidalCategory DistributiveCategory
+
+open scoped MonoidalCategory
+
+open HasCommRel
+
+namespace Term
+
+variable {φ : Type _} {α : Type _} {ε : Type _} [S : Signature φ α ε]
+         {C : Type _} [Category C] [PremonoidalCategory C] [CC : ChosenFiniteCoproducts C]
+        [BraidedCategory' C] [Iterate C] [E : Elgot2 C ε] [Model φ α ε C]
+
+class RWS.Valid (R : RWS φ α) (C : Type _)
+  [Category C] [PremonoidalCategory C] [CC : ChosenFiniteCoproducts C]
+  [BraidedCategory' C] [Iterate C] [E : Elgot2 C ε] [Model φ α ε C]
+  : Prop where
+  den_eq {Γ A a b} (h : R Γ A a b) (Da : Γ ⊢ a : A) (Db : Γ ⊢ b : A) : Da.den (C := C) = Db.den
+
+instance RWS.instValidBot : Valid (φ := φ) ⊥ C where den_eq h := h.elim
+
+-- TODO: Requires coherence!
+-- theorem RWS.uniform.eq {R : RWS φ α} [R.Valid C] {Γ A a b} (h : uniform R Γ A a b)
+--   (Da : Γ ⊢ a : A) (Db : Γ ⊢ b : A) : Da.den (C := C) = Db.den := sorry
